



$$(1) m(a+bX) = a + b \cdot m(X)$$

$$y_i = a + bx_i$$

$$m(a+bX) = m(Y) = \frac{1}{N} \sum_{i=1}^N y_i = \frac{1}{N} \sum_{i=1}^N (a + bx_i) = \frac{1}{N} \left(\sum_{i=1}^N a \right) + \frac{b}{N} \sum_{i=1}^N x_i = a + b m(X)$$

$$(2) \text{cov}(X, X) = s^2$$

$$\text{cov}(X, X) = \frac{1}{N} \sum_{i=1}^N (x_i - m(X)) (x_i - m(X)) = \frac{1}{N} \sum_{i=1}^N (x_i - m(X))^2 = s^2$$

$$(3) \text{cov}(X, a+bY) = b \text{cov}(X, Y)$$

$$Z = a + bY \quad \text{so} \quad z_i = a + by_i$$

$$m(Z) = a + b m(Y)$$

$$\text{cov}(X, Z) = \frac{1}{N} \sum_{i=1}^N (x_i - m(X)) (z_i - m(Z)) = \frac{1}{N} \sum_{i=1}^N (x_i - m(X)) ((a + by_i) - (a + b m(Y)))$$

$$= \frac{1}{N} \sum_{i=1}^N (x_i - m(X)) \cdot b(y_i - m(Y)) = b \cdot \frac{1}{N} \sum_{i=1}^N (x_i - m(X)) (y_i - m(Y)) = b \text{cov}(X, Y)$$

$$(4) \text{cov}(a+bX, a+bY) = b^2 \text{cov}(X, Y)$$

$$U = a + bX$$

$$V = a + bY$$

$$u_i - m(U) = b(x_i - m(X))$$

$$v_i - m(V) = b(y_i - m(Y))$$

$$\text{cov}(U, V) = \frac{1}{N} \sum_{i=1}^N (u_i - m(U)) (v_i - m(V)) = \frac{1}{N} \sum_{i=1}^N (b(x_i - m(X))) (b(y_i - m(Y)))$$

$$= b^2 \cdot \frac{1}{N} \sum_{i=1}^N (x_i - m(X)) (y_i - m(Y)) = b^2 \text{cov}(X, Y)$$

$$Y = X$$

$$\text{cov}(bX, bX) = b^2 \text{cov}(X, X) = b^2 s^2$$

(5) Yes, for $b > 0$ because the transformation $x \mapsto a + bx$ is strictly increasing so it preserves order of the data.

Median is $Q_{0.5}$ so $a + b \text{med}(X)$

$$\text{IQR}(a+bX) = (a + b Q_{.75}(X)) - (a + b Q_{.25}(X)) = b(Q_{.75}(X) - Q_{.25}(X)) = b \text{IQR}(X)$$

$$(6) m(X^2) \neq (m(X))^2 \text{ and } M(\sqrt{X}) \neq \sqrt{m(X)}$$

$$X = \{0, 1\} \text{ then } m(X) = \frac{0+1}{2} = \frac{1}{2} \quad \sqrt{m(X)} = \sqrt{\frac{1}{2}} \approx 0.707$$

$$(m(X))^2 = \left(\frac{1}{2}\right)^2 = \frac{1}{4} \quad \text{so } m(\sqrt{X}) \neq \sqrt{m(X)}$$